
\begin{align*}
    \frac{T_2}{T_1}=\left(\frac{P_2}{P_1}\right)^\frac{\gamma-1}{\gamma} \\
    T_2=T_1\left(\frac{P_2}{P_1}\right)^\frac{\gamma-1}{\gamma} \\
    T_2=1400\text{K}\left(\frac{1}{8}\right)^\frac{1.4-1}{1.4} \\
    \fbox{$T_2=772.86$K}
\end{align*}


\begin{align*}
    \rho_1=\frac{P_1}{RT_1} \\
    \rho_1=\frac{810600\text{Pa}}{287\text{J/kgK}*1400\text{K}} \\
    \rho_1=2.017\text{kg/m}^3
\end{align*}

\begin{align*}
    V_1=M_1\sqrt{\gamma RT_1} \\
    V_1=0.3\sqrt{1.4*287\text{J/kgK}*1400\text{K}} \\
    V_1=225\text{m/s}
\end{align*}

\begin{align*}
    \dot{m}=\rho_1 V_1 A_1 \\
    A_1=\frac{\dot{m}}{\rho_1V_1} \\
    A_1=\frac{100\text{kg/s}}{2.017\text{kg/m}^3\cdot 225\text{m/s}} \\
    \fbox{$A_1=0.22$m$^2$}
\end{align*}


\begin{align*}
    \frac{P_0}{P}=\left(1+\frac{\gamma-1}{2}M^2\right)^\frac{\gamma}{\gamma-1} \\
    P_0=P_1\left(1+\frac{\gamma-1}{2}M_1^2\right)^\frac{\gamma}{\gamma-1} \\
    P_0=862827.2\text{Pa}
\end{align*}

\begin{align*}
    \frac{P_0}{P}=\frac{862827.2}{101325}=8.52
\end{align*}


\begin{align*}
    T_{01}=T_1\left(1+\frac{\gamma-1}{2}M_1^2\right) \\
    T_{01}=1450.4\text{K}
\end{align*}

\begin{align*}
    M_2=\sqrt{\left(\frac{T_{01}}{T_2}-1\right)\frac{2}{\gamma-1}} \\
    M_2=2.1
\end{align*}

\begin{align*}
    \frac{A_1}{A^*}=\frac{1}{M_1}\left[\frac{2}{\gamma+1}\left(1+\frac{\gamma-1}{2}M_1^2
    \right)\right]^{\frac{\gamma+1}{2(\gamma-1)}} \\
    A^*=A_1/\frac{1}{M_1}\left[\frac{2}{\gamma+1}\left(1+\frac{\gamma-1}{2}M_1^2
    \right)\right]^{\frac{\gamma+1}{2(\gamma-1)}} \\
    A^*=0.108\text{m}^2
\end{align*}

\begin{align*}
    A_2=A^*\frac{1}{M_2}\left[\frac{2}{\gamma+1}\left(1+\frac{\gamma-1}{2}M_2^2
    \right)\right]^{\frac{\gamma+1}{2(\gamma-1)}} \\
    \fbox{$A_2=0.1984$m$^2$}
\end{align*}


\begin{align*}
    P_0=P_1\left(1+\frac{\gamma-1}{2}M_1^2\right)^\frac{\gamma}{\gamma-1} \\
    P_0=4\text{psia}\left(1+\frac{1.4-1}{2}2.5^2\right)^\frac{1.4}{1.4-1} \\
    P_0=68.3\text{psia}
\end{align*}

\begin{align*}
    T_0=T_1\left(1+\frac{\gamma-1}{2}M_1^2\right) \\
    T_0=(-55+459.67\text{R})\left(1+\frac{1.4-1}{2}2.5^2\right) \\
    T_0=910.5\text{K}
\end{align*}

\begin{align*}
    MFP=\sqrt{\frac{\gamma g_c}{R}}M_1\left(1+\frac{\gamma-1}{2}M_1^2\right)^
    {-\frac{\gamma+1}{2(\gamma-1)}} \\
    MFP=\sqrt{\frac{1.4(32.174\text{lbm-ft/lbf-s}^2)}{53.34\text{ft-lbf/lbm-R}}}\cdot 2.5\left(
    1+\frac{1.4-1}{2}2.5^2\right)^{-\frac{1.4+1}{2(1.4-1)}} \\
    MFP=0.202
\end{align*}

\begin{align*}
    \dot{m}=\frac{A_1P_0}{\sqrt{T_0}}MFP \\
    \dot{m}=\frac{1.5\text{ft}^268.3psia\frac{144si}{sf}}{\sqrt{910.5\text{R}}}(.202) \\
    \fbox{$\dot{m}=98.76$lbm/s}
\end{align*}

\begin{align*}
    P_2=P_0/\left(1+\frac{\gamma-1}{2}M_2^2\right)^\frac{\gamma}{\gamma-1} \\
    \fbox{$P_2=66.4$ psia}
    T_2=T_0/\left(1+\frac{\gamma-1}{2}M_2^2\right) \\
    \fbox{$T_2=903.3^\circ$R}
\end{align*}

\begin{align*}
    MFP=\sqrt{\frac{\gamma g_c}{R}}M_2\left(1+\frac{\gamma-1}{2}M_2^2\right)^
    {-\frac{\gamma+1}{2(\gamma-1)}} \\
    MFP=\sqrt{\frac{1.4(32.174\text{lbm-ft/lbf-s}^2)}{53.34\text{ft-lbf/lbm-R}}}\cdot 0.2\left(
    1+\frac{1.4-1}{2}0.2^2\right)^{-\frac{1.4+1}{2(1.4-1)}} \\
    MFP=0.179
\end{align*}

\begin{align*}
    A_2=\frac{\dot{m}\sqrt{T_0}}{MFP\cdot P_0} \\
    A_2=\frac{98.76\text{lbm/s}\sqrt{910.5\text{R}}}{0.179\cdot 68.3\text{psia}
    \frac{144\text{si}}{1\text{sf}}} \\
    \fbox{$A_2=1.693$ft$^2$}
\end{align*}


\begin{align*}
    T_{01}=T_1\left(1+\frac{\gamma-1}{2}M_1^2\right) \\
    T_{01}=260\left(1+\frac{1.4-1}{2}3^2\right) \\
    \fbox{$T_{01}=728$K}
\end{align*}

\begin{align*}
    P_{01}=P_1\left(1+\frac{\gamma-1}{2}M_1^2\right)^\frac{\gamma}{\gamma-1} \\
    P_{01}=20\left(1+\frac{1.4-1}{2}3^2\right)^\frac{1.4}{1.4-1} \\
    \fbox{$P_{01}=734.65$kPa}
\end{align*}

\begin{align*}
    T_2=T_1\left[1+\frac{2\gamma}{\gamma+1}(M_1^2-1)\right]\left[\frac{2+(\gamma-1)
    M_1^2}{(\gamma+1)M_1^2}\right] \\
    T_2=260\left[1+\frac{2\cdot 1.4}{2.4}(3^2-1)\right]\left[\frac{2+(0.4)3^2}
    {(2.4)3^2}\right] \\
    \fbox{$T_2=696.54$K}
\end{align*}

\begin{align*}
    P_2=P_1\left(1+\frac{2\gamma}{\gamma+1}(M_1^2-1)\right) \\
    P_2=20\left(1+\frac{2.8}{2.4}(3^2-1)\right) \\
    \fbox{$P_2=206.67$kPa}
\end{align*}

\begin{align*}
    M_2=\sqrt{\frac{1+\frac{\gamma-1}{2}M_1^2}{\gamma M_1^2-\frac{\gamma-1}{2}}} \\
    M_2=\sqrt{\frac{1+\frac{1.4-1}{2}3^2}{1.4\cdot 3^2-\frac{1.4-1}{2}}} \\
    M_2=0.4752
\end{align*}

\begin{align*}
    P_{02}=P_2\left(1+\frac{\gamma-1}{2}M_2^2\right)^\frac{\gamma}{\gamma-1} \\
    P_{02}=206.67\left(1+\frac{0.4}{2}0.4752^2\right)^\frac{1.4}{0.4} \\
    \fbox{$P_{02}=241.22$kPa}
\end{align*}


\begin{align*}
    \frac{T_{02}}{T_{01}}=\left(\frac{T_{02}}{T_{0}^*}\right)
    \left(\frac{T_{0}^*}{T_{01}}\right) \\
    \frac{T_{02}}{T_0^*}=\frac{T_{02}}{T_{01}}\frac{T_{0}^*}{T_{01}} \\
    \frac{T_{02}}{T_0^*}=\frac{998}{500}(1/0.34686) \\
    \frac{T_{02}}{T_0^*}=5.7545
\end{align*}

\begin{align*}
    q=c_p(T_{02}-T_{01}) \\
    T_{02}=q/c_p+T_{01} \\
    T_{02}=\frac{500\text{kJ/kg}}{1.004\text{kJ/kg-K}}+500\text{K} \\
    \fbox{$T_{02}=998$K}
\end{align*}

\begin{align*}
    \frac{P_{01}}{P_0^*}=1.1985 \\
    P_0^*=500.63\text{kPa}
\end{align*}

\begin{align*}
    \frac{P_{02}}{P_0^*}=1.1139 \\
    P_{02}=500.63(1.1139) \\
    \fbox{$P_{02}=557.65$kPa}
\end{align*}

\begin{align*}
    \frac{4c_fL}{D}=\frac{4(0.004)(8)}{1}=0.128
\end{align*}

\begin{align*}
    \frac{4c_fL_2^*}{D}=0.49080-0.128=0.3628
\end{align*}